Organize some parts of rings.

fowl/Is/Cancellative.v
@@ -3,35 +3,50 @@
 From Coq Require Import
   Logic.FunctionalExtensionality.
 From Maniunfold.Has Require Export
-  BinaryOperation.
+  NullaryOperation BinaryOperation.
 From Maniunfold.Is Require Export
   Injective.
 From Maniunfold.ShouldHave Require Import
   AdditiveNotations.
 
-(** This has the same shape as [mul_reg_l] and
-    a different shape from [add_reg_l]. *)
-
 Class IsCancelL (A : Type) (Hk : HasBinOp A) : Prop :=
-  cancel_l (x y z : A) (a : x + z = y + z) : x = y.
+  cancel_l (x y z : A) (a : z + x = z + y) : x = y.
 
-(** This has the same shape as [mul_reg_r]. *)
+(** This has the same shape as [add_reg_l]. *)
 
 Class IsCancelR (A : Type) (Hk : HasBinOp A) : Prop :=
-  cancel_r (x y z : A) (a : z + x = z + y) : x = y.
+  cancel_r (x y z : A) (a : x + z = y + z) : x = y.
 
 Class IsCancelLR (A : Type) (Hk : HasBinOp A) : Prop := {
   is_cancel_l :> IsCancelL _+_;
   is_cancel_r :> IsCancelR _+_;
 }.
 
-Module RFromL.
+(** This has the same shape as [mul_reg_l]. *)
+
+Class IsNonzeroCancelL (A : Type)
+  (Hx : HasNullOp A) (Hk : HasBinOp A) : Prop :=
+  nonzero_cancel_l (x y z : A) (f : z <> 0) (a : z + x = z + y) : x = y.
+
+(** This has the same shape as [mul_reg_r]. *)
+
+Class IsNonzeroCancelR (A : Type)
+  (Hx : HasNullOp A) (Hk : HasBinOp A) : Prop :=
+  nonzero_cancel_r (x y z : A) (f : z <> 0) (a : x + z = y + z) : x = y.
+
+Class IsNonzeroCancelLR (A : Type)
+  (Hx : HasNullOp A) (Hk : HasBinOp A) : Prop := {
+  is_nonzero_cancel_l :> IsNonzeroCancelL 0 _+_;
+  is_nonzero_cancel_r :> IsNonzeroCancelR 0 _+_;
+}.
+
+Module LFromR.
 
 Section Context.
 
 Context (A : Type) (Hk : HasBinOp A) `(!IsCancelL _+_).
 
-(** Flipped left cancellation is a right cancellation. *)
+(** Flipped right cancellation is a left cancellation. *)
 
 #[local] Instance is_cancel_r : IsCancelR (flip _+_).
 Proof.
@@ -46,15 +61,15 @@ End Context.
 
 #[export] Hint Resolve is_cancel_r : typeclass_instances.
 
-End RFromL.
+End LFromR.
 
-Module LFromR.
+Module RFromL.
 
 Section Context.
 
 Context (A : Type) (Hk : HasBinOp A) `(!IsCancelR _+_).
 
-(** Flipped right cancellation is a left cancellation. *)
+(** Flipped left cancellation is a right cancellation. *)
 
 #[local] Instance is_cancel_l : IsCancelL (flip _+_).
 Proof.
@@ -69,7 +84,7 @@ End Context.
 
 #[export] Hint Resolve is_cancel_l : typeclass_instances.
 
-End LFromR.
+End RFromL.
 
 Section Context.
 
@@ -77,23 +92,23 @@ Context (A : Type) (Hk : HasBinOp A).
 
 (** Cancellativity is just injectivity of partial applications. *)
 
-#[local] Instance cancel_l_is_inj `(!IsCancelL _+_) : IsInj _+_.
+#[local] Instance cancel_r_is_inj `(!IsCancelR _+_) : IsInj _+_.
 Proof.
   intros x y a.
   assert (z : A) by assumption.
   pose proof equal_f a z as a'.
-  apply cancel_l in a'.
+  apply cancel_r in a'.
   apply a'. Qed.
 
-#[local] Instance cancel_r_is_inj `(!IsCancelR _+_) : IsInj (flip _+_).
+#[local] Instance cancel_l_is_inj `(!IsCancelL _+_) : IsInj (flip _+_).
 Proof.
   intros x y a.
   assert (z : A) by assumption.
   pose proof equal_f a z as a'.
   unfold flip in a'.
-  apply cancel_r in a'.
+  apply cancel_l in a'.
   apply a'. Qed.
 
 End Context.
 
-#[export] Hint Resolve cancel_l_is_inj cancel_r_is_inj : typeclass_instances.
+#[export] Hint Resolve cancel_r_is_inj cancel_l_is_inj : typeclass_instances.
