fowl/Is/OneSortedCommutativeRing.v
@@ -2,13 +2,13 @@ From Maniunfold.Has Require Export
   Addition Zero Negation
   Multiplication One.
 From Maniunfold.Is Require Export
-  OneSortedRing Commutative.
+  Ring Commutative.
 
 (** Commutative ring. *)
 
 Class IsCommRing (A : Type)
   `(HasAdd A) `(HasZero A) `(HasNeg A)
   `(HasMul A) `(HasOne A) : Prop := {
-  A_add_zero_neg_mul_one_is_ring :> IsRing add zero neg mul one;
+  A_add_zero_neg_mul_one_is_ring :> IsRing zero neg add one mul;
   A_mul_is_comm :> IsComm mul;
 }.
