fowl/Is/Ring.v
@@ -1,0 +1,165 @@
+(** * Ring *)
+
+From Coq Require Import
+  Logic.Eqdep_dec.
+From Maniunfold Require Export
+  TypeclassTactics.
+From Maniunfold.Has Require Export
+  Zero Negation Addition One Multiplication.
+From Maniunfold.Is Require Export
+  Group Commutative Monoid Distributive
+  Cancellative Absorbing OneSortedSignedAbsorbing OneSortedBinaryCommutative
+  OneSortedBinaryCrossing OneSortedBinarySplitCancellative
+  OneSortedDegenerate OneSortedSemiring OneSortedGradedRing
+  Unital.
+From Maniunfold.ShouldHave Require Import
+  AdditiveNotations ArithmeticNotations.
+From Maniunfold.ShouldHave Require
+  OneSortedGradedAdditiveNotations OneSortedGradedArithmeticNotations.
+
+Class IsRing (A : Type)
+  (Hx : HasZero A) (Hf : HasNeg A) (Hk : HasAdd A)
+  (Hy : HasOne A) (Hm : HasMul A) : Prop := {
+  is_grp :> IsGrp 0 -_ _+_;
+  is_comm :> IsComm _+_;
+  is_mon :> IsMon 1 _*_;
+  is_distr_l_r :> IsDistrLR _*_ _+_;
+}.
+
+Section Context.
+
+Context (A : Type) `(IsRing A).
+
+Import Zero.Subclass Negation.Subclass Addition.Subclass
+  One.Subclass Multiplication.Subclass.
+
+Ltac conversions := typeclasses
+  convert null_op into zero and un_op into neg and bin_op into add or
+  convert null_op into one and bin_op into mul.
+
+#[local] Instance is_absorb_elem_l : IsAbsorbElemL 0 _*_.
+Proof with conversions.
+  intros x.
+  apply (cancel_r (0 * x) 0 (1 * x))...
+  rewrite <- (distr_r 0 1 x).
+  rewrite (unl_bin_op_l 1).
+  rewrite (unl_bin_op_l (1 * x)).
+  reflexivity. Qed.
+
+#[local] Instance is_absorb_elem_r : IsAbsorbElemR 0 _*_.
+Proof with conversions.
+  intros x.
+  apply (cancel_r (x * 0) 0 (x * 1))...
+  rewrite <- (distr_l x 0 1).
+  rewrite (unl_bin_op_l 1).
+  rewrite (unl_bin_op_l (x * 1)).
+  reflexivity. Qed.
+
+#[local] Instance is_absorb_elem_l_r : IsAbsorbElemLR 0 _*_.
+Proof. split; typeclasses eauto. Qed.
+
+Theorem neg_mul_one_l_sgn_absorb (x : A) : (- 1) * x = - x.
+Proof with conversions.
+  apply (cancel_l ((- 1) * x) (- x) (1 * x))...
+  rewrite <- (distr_r 1 (- 1) x).
+  rewrite (inv_r 1)...
+  rewrite (absorb_elem_l x).
+  rewrite (unl_bin_op_l x).
+  rewrite (inv_r x)...
+  reflexivity. Qed.
+
+Global Instance neg_mul_one_is_l_sgn_absorb : IsLSgnAbsorb neg mul one.
+Proof. exact @neg_mul_one_l_sgn_absorb. Qed.
+
+Theorem neg_mul_one_r_sgn_absorb (x : A) : x * (- 1) = - x.
+Proof with conversions.
+  apply (cancel_l (x * (- 1)) (- x) (x * 1))...
+  rewrite <- (distr_l x 1 (- 1)).
+  rewrite (inv_r 1)...
+  rewrite (absorb_elem_r x).
+  rewrite (unl_bin_op_r x).
+  rewrite (inv_r x)...
+  reflexivity. Qed.
+
+Global Instance neg_mul_one_is_r_sgn_absorb : IsRSgnAbsorb neg mul one.
+Proof. exact @neg_mul_one_r_sgn_absorb. Qed.
+
+Global Instance neg_mul_one_is_sgn_absorb : IsSgnAbsorb neg mul one.
+Proof. split; typeclasses eauto. Qed.
+
+Theorem neg_mul_l_bin_comm (x y : A) : - (x * y) = x * (- y).
+Proof with conversions.
+  rewrite <- (r_sgn_absorb (x * y)).
+  rewrite <- (assoc x y (- 1))...
+  rewrite r_sgn_absorb.
+  reflexivity. Qed.
+
+Global Instance neg_mul_is_l_bin_comm : IsLBinComm neg mul.
+Proof. exact @neg_mul_l_bin_comm. Qed.
+
+Theorem neg_mul_r_bin_comm (x y : A) : - (x * y) = (- x) * y.
+Proof with conversions.
+  rewrite <- (l_sgn_absorb (x * y)).
+  rewrite (assoc (- 1) x y)...
+  rewrite l_sgn_absorb.
+  reflexivity. Qed.
+
+Global Instance neg_mul_is_r_bin_comm : IsRBinComm neg mul.
+Proof. exact @neg_mul_r_bin_comm. Qed.
+
+Global Instance neg_mul_is_bin_comm : IsBinComm neg mul.
+Proof. split; typeclasses eauto. Qed.
+
+Theorem neg_mul_bin_crs (x y : A) : (- x) * y = x * (- y).
+Proof with conversions.
+  rewrite <- (l_bin_comm x y).
+  rewrite <- (r_bin_comm x y).
+  reflexivity. Qed.
+
+Global Instance neg_mul_is_bin_crs : IsBinCrs neg mul.
+Proof. exact @neg_mul_bin_crs. Qed.
+
+Theorem neg_mul_bin_spt_cancel (x y : A) : (- x) * (- y) = x * y.
+Proof with conversions.
+  rewrite <- (r_bin_comm x (- y)).
+  rewrite <- (l_bin_comm x y).
+  rewrite (invol (x * y)).
+  reflexivity. Qed.
+
+Global Instance neg_mul_is_bin_spt_cancel : IsBinSptCancel neg mul.
+Proof. exact @neg_mul_bin_spt_cancel. Qed.
+
+Global Instance add_zero_mul_one_is_semiring : IsSemiring add zero mul one.
+Proof. split; typeclasses eauto. Qed.
+
+Theorem one_zero_degen (x : A) (e : 1 = 0) : x = 0.
+Proof with conversions.
+  pose proof distr_l x 0 1 as e'.
+  rewrite unl_bin_op_l in e'. rewrite unl_bin_op_r in e' at 1. rewrite e in e'.
+  repeat rewrite absorb_elem_r in e'. rewrite unl_bin_op_r in e'. apply e'. Qed.
+
+Global Instance one_zero_is_degen : IsDegen zero one.
+Proof. exact @one_zero_degen. Qed.
+
+(** TODO Clean up. *)
+
+Global Instance integral_domain_thing
+  (a : forall x y : A, x * y = 0 -> x = 0 \/ y = 0) : IsNonzeroCancelL 0 _*_.
+Proof with conversions.
+  intros x y z f e.
+  typeclasses convert null_op into zero and bin_op into mul.
+  assert (e' : z * x + - (z * y) = 0).
+  { rewrite e.
+    rewrite (inv_r (z * y))...
+    reflexivity. }
+  rewrite l_bin_comm in e'.
+  rewrite <- distr_l in e'.
+  apply a in e'.
+  destruct e' as [e' | e'].
+  - congruence.
+  - apply (cancel_r x y (- y))...
+    rewrite e'.
+    rewrite (inv_r y)...
+    reflexivity. Qed.
+
+End Context.
