fowl/Is/TwoSortedAlgebra.v
@@ -3,7 +3,7 @@ From Maniunfold.Has Require Export
   Multiplication One
   Action.
 From Maniunfold.Is Require Export
-  OneSortedRing TwoSortedBimodule TwoSortedBilinearOperator.
+  Ring TwoSortedBimodule TwoSortedBilinearOperator.
 
 (** Noncommutative nonunital nonassociative algebra over a noncommutative ring.
     The ring is carried by [A] and the algebra by [B].
@@ -15,7 +15,7 @@ Class IsAlg (A B : Type)
   `(HasAdd B) `(HasZero B) `(HasNeg B)
   `(HasMul B)
   `(HasActL A B) `(HasActR A B) : Prop := {
-  A_add_zero_neg_mul_one_is_ring :> IsRing add zero neg mul one;
+  A_zero_neg_add_one_mul_is_ring :> IsRing zero neg add one mul;
   A_B_add_zero_neg_mul_one_add_zero_neg_act_l_act_r_is_two_bimod :>
     IsTwoBimod add zero neg mul one add zero neg (act_l (A := A) (B := B)) act_r;
   A_B_add_zero_neg_mul_one_add_zero_neg_mul_act_l_act_r_is_bilin_op :>
