fowl/Is/TwoSortedRightModule.v
@@ -3,7 +3,7 @@ From Maniunfold.Has Require Export
   Multiplication One
   Action.
 From Maniunfold.Is Require Export
-  OneSortedRing OneSortedAbelianGroup
+  Ring OneSortedAbelianGroup
   TwoSortedRightLeftDistributive TwoSortedRightCompatible
   TwoSortedRightUnital TwoSortedRightRightDistributive.
 
@@ -15,7 +15,7 @@ Class IsRMod (A B : Type)
   `(HasMul A) `(HasOne A)
   `(HasAdd B) `(HasZero B) `(HasNeg B)
   `(HasActR A B) : Prop := {
-  A_add_zero_neg_mul_one_is_ring :> IsRing add zero neg mul one;
+  A_zero_neg_add_one_mul_is_ring :> IsRing zero neg add one mul;
   B_add_zero_neg_is_ab_grp :> IsAbGrp add zero neg;
   A_B_add_add_act_r_is_two_r_distr_l :> IsTwoRDistrL add add act_r;
   A_B_mul_act_r_is_r_compat :> IsRCompat mul act_r;
