fowl/Provides/UnitTheorems.v
@@ -1,7 +1,7 @@
 From Maniunfold.Is Require Export
   OneSortedAbelianGroup Semigroup
   Monoid OneSortedSemiring
-  OneSortedRing OneSortedCommutativeSemigroup OneSortedCommutativeMonoid
+  Ring OneSortedCommutativeSemigroup OneSortedCommutativeMonoid
   OneSortedCommutativeSemiring OneSortedCommutativeRing.
 
 Ltac eautodestruct :=
@@ -140,8 +140,8 @@ Global Instance unit_add_zero_mul_one_is_comm_semiring :
   IsCommSemiring add zero mul one.
 Proof. split; typeclasses eauto. Defined.
 
-Global Instance unit_add_zero_neg_mul_one_is_ring :
-  IsRing add zero neg mul one.
+Global Instance unit_zero_neg_add_one_mul_is_ring :
+  IsRing zero neg add one mul.
 Proof. split; typeclasses eauto. Defined.
 
 Global Instance unit_mul_is_comm : IsComm mul.
